generalized adequacy to apply to multi-threaded initial states

heap_lang/simulation_adequacy.v
@@ -23,6 +23,71 @@ Section adequacy.
               WP e1 @ s; locale_of [] e1; ⊤ {{ _, em_thread_post 0%nat (em_GS0 := heap_fairnessGS)}} ∗
                                             rel_always_holds0 R s state_interp (fun _ => em_thread_post 0%nat (em_GS0 := heap_fairnessGS)) e1 σ1 s1)). 
 
+  Definition wp_premise_multiple
+    `{EM: ExecutionModel heap_lang M}
+    (Σ: gFunctors)
+    (s: stuckness) es σ1 (s1: mstate M)
+    (R: execution_trace heap_lang → auxiliary_trace M → Prop)
+    (p: em_init_param)
+    := 
+    (∀ `{Hinv : @heapGS Σ M EM} ,
+        ⊢ (([∗ map] l ↦ v ∈ heap σ1, pointsto l (DfracOwn 1) v) ∗
+             em_init_resource s1 p (em_GS0 := heap_fairnessGS)
+           ={⊤}=∗
+              let Φs := map (fun i _ => em_thread_post i%nat (em_GS0 := heap_fairnessGS)) (seq 0 (length es)) in
+              wptp s es Φs ∗
+              rel_always_holds s Φs R (es, σ1) s1)).
+
+  Lemma wp_premise_single `{EM: ExecutionModel heap_lang M} Σ
+    s e1 σ1 s1 R p:
+    wp_premise Σ s e1 σ1 s1 R p -> wp_premise_multiple Σ s [e1] σ1 s1 R p.
+  Proof using.
+    rewrite /wp_premise /wp_premise_multiple.
+    iIntros "%WP1 % [HEAP INIT]".
+    iMod (WP1 Hinv with "[$HEAP $INIT]") as "[WP1 RAH]".
+    iFrame. set_solver.
+  Qed.
+
+  Theorem strong_simulation_adequacy_general_multiple
+    `{hPre: @heapGpreS Σ M EM} (s: stuckness) (es : list expr) σ1 (s1: M)
+    (R: execution_trace heap_lang → auxiliary_trace M → Prop)
+    (p: em_init_param)    
+    :
+    length es ≥ 1 ->
+    rel_finitary R →
+    em_is_init_st (es, σ1) s1 ->
+    em_valid_state_evolution_fairness {tr[ (es, σ1) ]} {tr[ s1 ]} ->
+    (wp_premise_multiple Σ s es σ1 s1 R p) ->
+    continued_simulation R (trace_singleton (es, σ1)) (trace_singleton s1).
+  Proof.
+    intros LEN Hfin INIT VALID1 H.
+    apply (wp_strong_adequacy_multiple_with_trace_inv heap_lang M Σ s); try done.
+
+    iIntros (?) "".
+
+    iMod (gen_heap_init (heap σ1)) as (genheap)" [Hgen [Hσ _]]".  
+    iMod (em_initialization _ s1 (es, σ1) p) as (fGS) "[LM_INIT MSI]"; [done| ].
+    Unshelve. 2: by apply hPre. 
+
+    set (distG := {| heap_fairnessGS := (fGS: (em_GS Σ (ExecutionModel := EM))) |}).
+    iPoseProof (H distG) as "Hwp". clear H.
+    
+    iExists state_interp, (λ _ _, ⌜ True ⌝%I), _, (fun τ _ => em_thread_post τ).
+    iSplitR.
+    { unfold config_wp. iIntros "!>!>" (???????) "?". done. }
+
+    iSpecialize ("Hwp" with "[Hσ LM_INIT]"); [by iFrame| ]. 
+    iDestruct "Hwp" as ">[Hwp H]". 
+    iModIntro. iFrame "Hwp Hgen MSI".
+
+    (* TODO: make a lemma *)
+    iIntros (??????????) "SI POSTS".
+    rewrite /rel_always_holds. iDestruct ("H" with "[][][][][][][] SI POSTS") as "R".
+    all: try by done.
+    iSplit. 
+    - iModIntro; iIntros "[$ ?]"; done.
+    - eauto. 
+  Qed.
 
   Theorem strong_simulation_adequacy_general
     `{hPre: @heapGpreS Σ M EM} (s: stuckness) (e1 : expr) σ1 (s1: M)
@@ -35,28 +100,44 @@ Section adequacy.
     (wp_premise Σ s e1 σ1 s1 R p) ->
     continued_simulation R (trace_singleton ([e1], σ1)) (trace_singleton s1).
   Proof.
-    intros Hfin INIT VALID1 H.
-    intros. apply (wp_strong_adequacy heap_lang M Σ s); [done| ]. 
-    iIntros (?) "".
+    intros. eapply strong_simulation_adequacy_general_multiple.
+    1-4: by eauto.
+    apply wp_premise_single. eauto. 
+  Qed.
 
-    iMod (gen_heap_init (heap σ1)) as (genheap)" [Hgen [Hσ _]]".  
-    iMod (em_initialization _ s1 ([e1], σ1) p) as (fGS) "[LM_INIT MSI]"; [done| ].
-    Unshelve. 2: by apply hPre. 
-
-    set (distG := {| heap_fairnessGS := (fGS: (em_GS Σ (ExecutionModel := EM))) |}).
-    iPoseProof (H distG) as "Hwp". clear H.
-    
-    iExists state_interp, (fun _ => em_thread_post 0%nat), fork_post.
-    iSplitR.
-    { unfold config_wp. iIntros "!>!>" (???????) "?". done. }
-
-    iSpecialize ("Hwp" with "[Hσ LM_INIT]"); [by iFrame| ]. 
-    iDestruct "Hwp" as ">[Hwp H]". 
-    iModIntro. iFrame.
+  Theorem strong_simulation_adequacy_inftraces_multiple Σ
+    `{hPre: @heapGpreS Σ M EM} (s: stuckness) 
+    (es : list expr) σ1 (s1: M)
+    (R: execution_trace heap_lang → auxiliary_trace M → Prop)
+    (p: em_init_param)
+    (iex : inf_execution_trace heap_lang)
+    (Hvex : valid_inf_exec (trace_singleton (es, σ1)) iex)
+    :
+    length es ≥ 1 ->
+    rel_finitary R →
+    em_is_init_st (es, σ1) s1 ->
+    (wp_premise_multiple Σ s es σ1 s1 R p) ->
+    exists iatr,
+      @valid_inf_system_trace _ M
+        (@continued_simulation
+           heap_lang
+           M
+           R)
+        (trace_singleton (es, σ1))
+        (trace_singleton s1)
+        iex
+        iatr.
+  Proof.
+    intros LEN Hfin Hwp.
+    eexists.
+    eapply produced_inf_aux_trace_valid_inf.
+    Unshelve.
+    - econstructor.
+    - eapply (strong_simulation_adequacy_general_multiple s) => //.
+    - done.
   Qed.
 
   Theorem strong_simulation_adequacy_inftraces Σ
-
     `{hPre: @heapGpreS Σ M EM} (s: stuckness) 
     (e1 : expr) σ1 (s1: M)
     (R: execution_trace heap_lang → auxiliary_trace M → Prop)
@@ -78,24 +159,20 @@ Section adequacy.
         iex
         iatr.
   Proof.
-    intros Hfin Hwp.
-    eexists.
-    eapply produced_inf_aux_trace_valid_inf.
-    Unshelve.
-    - econstructor.
-    - eapply (strong_simulation_adequacy_general s) => //.
-    - done.
+    intros. eapply strong_simulation_adequacy_inftraces_multiple.
+    1-5: by eauto.
+    by eapply wp_premise_single. 
   Qed.
 
-  Theorem strong_simulation_adequacy_traces Σ
+  Theorem strong_simulation_adequacy_traces_multiple Σ
     `{hPre: @heapGpreS Σ M EM} (s: stuckness) 
-    (e1 : expr) σ1 (s1: M)
+    (es: list expr) σ1 (s1: M)
     (R: execution_trace heap_lang → auxiliary_trace M → Prop)
     (p: em_init_param)
 
     (extr : heap_lang_extrace)
     (Hvex : extrace_valid extr)
-    (Hexfirst : trfirst extr = ([e1], σ1))
+    (Hexfirst : trfirst extr = (es, σ1))
 
     (valid_step: cfg heap_lang -> olocale heap_lang → cfg heap_lang → 
                  mstate M → mlabel M → mstate M -> Prop)
@@ -111,14 +188,15 @@ Section adequacy.
     (R_STEP: forall extr mtr, R extr mtr -> valid_state_evolution_fairness valid_step extr mtr)
 
     :
+    length es ≥ 1 ->
     rel_finitary R →
-    em_is_init_st ([e1], σ1) s1 ->
-    (wp_premise Σ s e1 σ1 s1 R p) ->
+    em_is_init_st (es, σ1) s1 ->
+    (wp_premise_multiple Σ s es σ1 s1 R p) ->
     ∃ (mtr : trace (mstate M) (mlabel M)), 
       traces_match lbl_rel state_rel locale_step (@mtrans M) extr mtr /\
       trfirst mtr = s1. 
   Proof.
-    intros Hfin INIT Hwp.
+    intros ? Hfin INIT Hwp.
     have [iatr MATCH] : exists iatr,
         @valid_inf_system_trace
           heap_lang M
@@ -126,13 +204,13 @@ Section adequacy.
              heap_lang
              M
              R)
-          (trace_singleton ([e1], (trfirst extr).2))
+          (trace_singleton (es, (trfirst extr).2))
           (trace_singleton s1)
           (from_trace extr)
           iatr.
-    { eapply (strong_simulation_adequacy_inftraces _ s); eauto.
-      eapply from_trace_preserves_validity; eauto; first econstructor.
-      all: by rewrite Hexfirst. }
+    { eapply (strong_simulation_adequacy_inftraces_multiple _ s); eauto.
+      1: eapply from_trace_preserves_validity; eauto; first econstructor.
+      all: try by rewrite Hexfirst. }
     rewrite Hexfirst in MATCH. simpl in *. 
     exists (to_trace s1 iatr).
 
@@ -168,6 +246,42 @@ Section adequacy.
         using the notion of traces_match (MATCH hypothesis). *)
 
     apply MATCH. 
+  Qed.
+
+  Theorem strong_simulation_adequacy_traces Σ
+    `{hPre: @heapGpreS Σ M EM} (s: stuckness) 
+    (e1 : expr) σ1 (s1: M)
+    (R: execution_trace heap_lang → auxiliary_trace M → Prop)
+    (p: em_init_param)
+
+    (extr : heap_lang_extrace)
+    (Hvex : extrace_valid extr)
+    (Hexfirst : trfirst extr = ([e1], σ1))
+
+    (valid_step: cfg heap_lang -> olocale heap_lang → cfg heap_lang → 
+                 mstate M → mlabel M → mstate M -> Prop)
+    (state_rel: cfg heap_lang -> mstate M -> Prop)
+    (lbl_rel: olocale heap_lang -> mlabel M -> Prop)
+    (STEP_LBL_REL: forall c1 oζ c2 δ1 ℓ δ2,
+                 valid_step c1 oζ c2 δ1 ℓ δ2 ->
+                 lbl_rel oζ ℓ)
+    (STEP_MTRANS: forall c1 oζ c2 δ1 ℓ δ2,
+                 valid_step c1 oζ c2 δ1 ℓ δ2 ->
+                 mtrans δ1 ℓ δ2)
+    (R_ST: forall extr mtr, R extr mtr -> state_rel (trace_last extr) (trace_last mtr))
+    (R_STEP: forall extr mtr, R extr mtr -> valid_state_evolution_fairness valid_step extr mtr)
+
+    :
+    rel_finitary R →
+    em_is_init_st ([e1], σ1) s1 ->
+    (wp_premise Σ s e1 σ1 s1 R p) ->
+    ∃ (mtr : trace (mstate M) (mlabel M)), 
+      traces_match lbl_rel state_rel locale_step (@mtrans M) extr mtr /\
+      trfirst mtr = s1. 
+  Proof.
+    intros. eapply strong_simulation_adequacy_traces_multiple; last first.
+    { by eapply wp_premise_single. }
+    all: by eauto.     
   Qed.
   
 End adequacy.
